Simplify Vale.Arch.Heap slightly

vale/code/arch/Vale.Arch.Heap.fst
@@ -3,13 +3,11 @@ open Vale.Interop
 open Vale.Arch.HeapImpl
 friend Vale.Arch.HeapImpl
 
-let heap_down = down_mem
-
 let heap_impl = vale_heap_impl
 
 let heap_get hi = hi.mh
 
-let heap_new ih mh = ValeHeap mh (Ghost.hide ih)
-
 let heap_upd hi mh' =
   mi_heap_upd hi mh'
+
+let heap_of_interop ih = ValeHeap (down_mem ih) (Ghost.hide ih)
