vale/specs/hardware/Vale.Arch.Heap.fsti
@@ -6,16 +6,12 @@ open Vale.Interop.Heap_s
 // This module defines the heap interface, called heap_impl, seen by Vale.X64.Machine_Semantics_s.
 // The interface is a trusted specification, but its implementation is defined in untrusted code.
 
-val heap_down : down_mem_t
-
 val heap_impl : Type u#1
 
 val heap_get (hi:heap_impl) : machine_heap
 
-val heap_new (ih:interop_heap) (mh:machine_heap) : Pure heap_impl
-  (requires mh == heap_down ih)
-  (ensures fun hi -> heap_get hi == mh)
-
 val heap_upd (hi:heap_impl) (mh':machine_heap) : Pure heap_impl
   (requires is_machine_heap_update (heap_get hi) mh')
   (ensures fun hi -> heap_get hi == mh')
+
+val heap_of_interop (ih:interop_heap) : GTot heap_impl
